Stage wip

proofs/Vector.v
@@ -6,6 +6,7 @@ Import ListNotations.
 From Coq Require Import Omega.
 From Coq Require Import Logic.FunctionalExtensionality.
 From Coq Require Import Program.Wf.
+From Coq Require Import Bool.Bool.
 
 From RRB Require Import Prelude.
 From RRB Require Import Crush.
@@ -83,6 +84,11 @@ Fixpoint vec_length {A : Set} (tr : @vector A) : nat :=
 Definition vec_length_order {A : Set} (tr1 tr2 : @vector A) :=
   vec_length tr1 < vec_length tr2.
 
+Lemma vec_length_node_elems {A : Set} :
+  forall (tr : @vector A) (ht : height) (szs : list size) (trs : list vector) (tr2 : vector),
+    tr = Node ht szs trs -> In tr2 trs -> vec_length tr2 < vec_length tr.
+  Admitted.
+
 Hint Constructors Acc.
 
 Lemma vec_length_order_wf' :
@@ -158,123 +164,42 @@ Definition indexInNode {A : Set}
                   Some (slot', idx')
   end.
 
-Program Fixpoint get {A : Set}
-  (tr : @vector A) (idx : nat) (default : A) {measure (vec_length tr)} : A :=
-  match tr with
-  | Leaf _ ns => if idx <? length ns
-                 then strong_nth idx ns _
-                 else default
-  | Node ht szs trs =>
-    match trs with
-    | [] => default
-    | a :: rst => match @indexInNode A ht szs idx  with
-                  | Some (slot' , idx') => get (strong_nth slot' trs _) idx' default
-                  | None => default
-                  end
-    end
-  end.
-   Admit Obligations.
-
-(*
-
-Verified lookup, WIP.
-
-(* Not using bit operations for now *)
-Definition index_of (ht : height) (i : nat) : nat :=
-  (i / (m ^ ht)) mod m.
-
-Lemma index_of_lt_m {A : Set} : forall (ht i : nat), m > 0 -> index_of ht i < m.
-Proof.
-  intros. unfold index_of. unfold modulo. destruct m.
-  + apply H.
-  + omega.
-Qed.
-
-Axiom nooo : forall {A : Set}
-  (ht : nat) (szs : list size) (trs : list (@vector A)) (tr : @vector A) (idx : nat),
-  (tr = Node ht szs trs) -> (idx < vec_length tr) -> index_of ht idx < length szs.
-
-Fixpoint check_slot_default
-  (sz_js : list (nat * nat)) (idx : nat) (default : nat) : nat :=
-  match sz_js with
-  | [] => default
-  | (sz , j) :: rst => if sz <? idx
-                       then check_slot_default rst idx j
-                       else j
-  end.
-
-Definition check_slot' :
-  forall (sz_js : list (nat * nat)) (idx : nat), sz_js <> [] -> nat.
-  refine (fix f (sz_js : list (nat * nat)) (idx : nat) :=
-              match sz_js with
-              | [] => fun pf  => _
-              | (sz , j) :: rst =>
-                  fun _ => check_slot_default rst idx j
-              end).
-    congruence.
-Defined.
-
-Definition check_slot
-  (s : { sz_js : list (nat * nat) | sz_js <> [] }) (idx : nat) : nat :=
-  check_slot' (proj1_sig s) idx (proj2_sig s).
-
-(*
-
-Want to prove:
-
-    (1) slot = index_of ht idx and slot < length szs
-
-    (2) slot' = check_slot sz_js idx and slot' < length szs
-
-We know:
-
-    (1) forall tr = Node ht szs trs, length szs = length trs.
-
-*)
-
-Definition indexInNode : forall {A : Set}
-  (ht : height) (trs : list (@vector A)) (szs : list size)
-  (tr : vector) (tr_node : tr = Node ht szs trs) (szs_not_nil : szs <> []) (idx : nat),
-  idx < (@vec_length A tr) -> (nat * nat).
-  refine (fun A ht trs szs tr tr_node szs_not_nil idx idx_lt_vec_len =>
-            let slot    := index_of ht idx in
-            let sz_js_1 := combine szs (seq 0 (length szs)) in
-            let sz_js   := skipn slot sz_js_1 in
-            (match sz_js as sz_js' return sz_js = sz_js' -> (nat * nat) with
-             | [] => fun sz_js_nil => _
-             | a :: b =>
-               fun _ =>
-                 let slot' := check_slot (exist _ (a :: b) (cons_not_nil a b)) idx in
-                 let idx' := idx - (if eqb slot' 0
-                                    then 0
-                                    else strong_nth szs (slot' - 1) _)
-                 in (slot' , idx')
-             end) (eq_refl sz_js)).
-  (* sz_js <> [] *)
-  + assert(slot_lt : slot < length (combine szs (seq 0 (length szs)))).
-    { rewrite combine_length. rewrite seq_length. rewrite min_eq.
-      apply nooo with trs tr. apply tr_node. apply idx_lt_vec_len. }
-  (*   assert (length_sz_js_not_O : length sz_js_1 <> 0). *)
-  (*   { subst. unfold sz_js_1. rewrite combine_length. rewrite seq_length. *)
-  (*     rewrite min_eq. apply length_zero_iff_nil. apply szs_not_nil. } *)
-  (*   apply length_not_zero_inv in length_sz_js_not_O. *)
+Definition get' {A : Set} (default : A) : (@vector A) -> nat -> A.
+  refine (Fix vec_length_order_wf
+           (fun _ => nat -> A)
+           (fun (tr : @vector A)
+                (get' : forall (tr' : @vector A), vec_length_order tr' tr -> nat -> A) =>
+              fun idx =>
+              (match tr as tr' return tr = tr' -> A with
+               | Leaf _ ns => fun tr_is_leaf =>
+                                if idx <? length ns
+                                then nth idx ns default
+                                else default
+               | Node ht szs trs =>
+                 fun tr_is_node =>
+                 (match trs as trs' return trs = trs' -> A with
+                 | [] => fun _ => default
+                 | a :: rst =>
+                   fun trs_not_nil =>
+                     match @indexInNode A ht szs idx  with
+                     | Some (slot' , idx') =>
+                       let node := strong_nth slot' trs _
+                       in get' node _ idx
+                     | None => default
+                     end
+                 end) (eq_refl trs)
+               end) (eq_refl tr))).
+  (* vec_length_order node tr *)
+  + rewrite tr_is_node. apply vec_length_node_elems with ht szs trs.
+    reflexivity. rewrite trs_not_nil.
+    (* apply (strong_nth_In slot' (a :: rst) node _). *)
   Admitted.
 
-Definition get {A : Set}
-   (tr : vector) (s : { idx : nat | (idx < @vec_length A tr) }) (default : A) : A.
-  refine ((match tr as tr' return tr = tr' -> A with
-           | Leaf szs ns => match s with
-                            | exist _ idx pf => fun tr => strong_nth ns idx _
-                            end
-           | Node ht szs trs => fun _ => default
-           end) (eq_refl tr)).
-  (* tr = Leaf .. *)
-  + rewrite vec_length_leaves_sizes with _ szs ns in pf.
-    - apply pf.
-    - apply tr.
-Defined.
+Global Transparent get'.
 
-*)
+Definition get {A : Set}
+  (tr : @vector A) (idx : nat) (default : A) : A := get' default tr idx.
+
 
 (* ---------------------------------- *)
 (* -- Insert front/back               *)
@@ -296,43 +221,46 @@ Inductive tmp_pair {A : Set} : Set :=
 
 
 Definition tryBottom_back {A : Set} (v1 : A) : (@vector A) -> option (@vector A).
-  refine (Fix vec_length_order_wf (fun _ => option (@vector A))
-  (fun (tr : @vector A)
-       (try_bottom_back : forall (tr' : @vector A), vec_length_order tr' tr -> option (@vector A)) =>
-  match tr with
-  | Leaf szs ns =>
-    if length ns <? m
-    then Some (Leaf (szs ++ [1]) (ns ++ [v1]))
-    else None
-  | Node ht szs trs =>
-    (match trs as trs' return trs = trs' -> option (@vector A) with
-     | [] => fun _ => Some (Node ht [1] [mkLeafAtHeight (ht - 1) v1])
-     | t :: ts  =>
-       fun trs_not_nil =>
-         (match szs as szs' return szs = szs' -> option (@vector A) with
-          | [] => fun _ => None
-          | s :: ss =>
-            fun szs_not_nil =>
-              let node_to_try := strong_last trs _ in
-              match try_bottom_back node_to_try _ with
-              | mb_vec => match mb_vec with
-                          | Some has_v => let last_sz := strong_last szs _ in
-                                          let szs' := removelast szs ++ [1 + last_sz] in
-                                          let trs' := removelast trs ++ [has_v] in
-                                          Some (Node ht szs' trs')
-                          | None =>
-                            if length trs <? m
-                            then let branch  := mkLeafAtHeight (ht - 1) v1 in
-                                 let last_sz := strong_last szs _ in
-                                 let szs'    := szs ++ [1 + last_sz] in
-                                 let trs'    := trs ++ [branch]
-                                 in Some (Node ht szs' trs')
-                            else None
-                          end
-              end
-          end) (eq_refl szs)
-     end) (eq_refl trs)
-  end)).
+  refine (Fix vec_length_order_wf
+            (fun _ => option (@vector A))
+            (fun (tr : @vector A)
+                 (try_bottom_back : forall (tr' : @vector A), vec_length_order tr' tr -> option (@vector A)) =>
+               ((match tr as tr' return tr = tr' -> option (@vector A) with
+               | Leaf szs ns =>
+                 fun _ =>
+                 if length ns <? m
+                 then Some (Leaf (szs ++ [1]) (ns ++ [v1]))
+                 else None
+               | Node ht szs trs =>
+                 fun tr_is_Node =>
+                 (match trs as trs' return trs = trs' -> option (@vector A) with
+                  | [] => fun _ => Some (Node ht [1] [mkLeafAtHeight (ht - 1) v1])
+                  | t :: ts  =>
+                    fun trs_not_nil =>
+                      (match szs as szs' return szs = szs' -> option (@vector A) with
+                       | [] => fun _ => None
+                       | s :: ss =>
+                         fun szs_not_nil =>
+                           let node_to_try := strong_last trs _ in
+                           match try_bottom_back node_to_try _ with
+                           | mb_vec => match mb_vec with
+                                       | Some has_v => let last_sz := strong_last szs _ in
+                                                       let szs' := removelast szs ++ [1 + last_sz] in
+                                                       let trs' := removelast trs ++ [has_v] in
+                                                       Some (Node ht szs' trs')
+                                       | None =>
+                                         if length trs <? m
+                                         then let branch  := mkLeafAtHeight (ht - 1) v1 in
+                                              let last_sz := strong_last szs _ in
+                                              let szs'    := szs ++ [1 + last_sz] in
+                                              let trs'    := trs ++ [branch]
+                                              in Some (Node ht szs' trs')
+                                         else None
+                                       end
+                           end
+                       end) (eq_refl szs)
+                  end) (eq_refl trs)
+               end) (eq_refl tr) ))).
   Unshelve.
   (* szs <> [] *)
   + rewrite szs_not_nil. apply (cons_not_nil s ss).
@@ -340,7 +268,11 @@ Definition tryBottom_back {A : Set} (v1 : A) : (@vector A) -> option (@vector A)
   (* trs <> [] *)
   + rewrite trs_not_nil. apply (cons_not_nil t ts).
   (* vec_length node_to_try < vec_length trs *)
-  + unfold vec_length_order. Admitted.
+  + unfold vec_length_order. rewrite tr_is_Node. rewrite trs_not_nil.
+    assert (H: In node_to_try (t :: ts)).
+    { apply (strong_last_In (t :: ts) node_to_try (cons_not_nil t ts)).
+      apply node_to_try. }
+    Admitted.
 
 Fixpoint tryBottom_front {A : Set} (v1 : A) (tr : @vector A) : option (@vector A) :=
   match tr with
