proofs/WIP.v
@@ -1,0 +1,155 @@
+(*
+
+Verified lookup, WIP.
+
+(* Not using bit operations for now *)
+Definition index_of (ht : height) (i : nat) : nat :=
+  (i / (m ^ ht)) mod m.
+
+Lemma index_of_lt_m {A : Set} : forall (ht i : nat), m > 0 -> index_of ht i < m.
+Proof.
+  intros. unfold index_of. unfold modulo. destruct m.
+  + apply H.
+  + omega.
+Qed.
+
+Axiom nooo : forall {A : Set}
+  (ht : nat) (szs : list size) (trs : list (@vector A)) (tr : @vector A) (idx : nat),
+  (tr = Node ht szs trs) -> (idx < vec_length tr) -> index_of ht idx < length szs.
+
+Fixpoint check_slot_default
+  (sz_js : list (nat * nat)) (idx : nat) (default : nat) : nat :=
+  match sz_js with
+  | [] => default
+  | (sz , j) :: rst => if sz <? idx
+                       then check_slot_default rst idx j
+                       else j
+  end.
+
+Definition check_slot' :
+  forall (sz_js : list (nat * nat)) (idx : nat), sz_js <> [] -> nat.
+  refine (fix f (sz_js : list (nat * nat)) (idx : nat) :=
+              match sz_js with
+              | [] => fun pf  => _
+              | (sz , j) :: rst =>
+                  fun _ => check_slot_default rst idx j
+              end).
+    congruence.
+Defined.
+
+Definition check_slot
+  (s : { sz_js : list (nat * nat) | sz_js <> [] }) (idx : nat) : nat :=
+  check_slot' (proj1_sig s) idx (proj2_sig s).
+
+(*
+
+Want to prove:
+
+    (1) slot = index_of ht idx and slot < length szs
+
+    (2) slot' = check_slot sz_js idx and slot' < length szs
+
+We know:
+
+    (1) forall tr = Node ht szs trs, length szs = length trs.
+
+*)
+
+Definition indexInNode : forall {A : Set}
+  (ht : height) (trs : list (@vector A)) (szs : list size)
+  (tr : vector) (tr_node : tr = Node ht szs trs) (szs_not_nil : szs <> []) (idx : nat),
+  idx < (@vec_length A tr) -> (nat * nat).
+  refine (fun A ht trs szs tr tr_node szs_not_nil idx idx_lt_vec_len =>
+            let slot    := index_of ht idx in
+            let sz_js_1 := combine szs (seq 0 (length szs)) in
+            let sz_js   := skipn slot sz_js_1 in
+            (match sz_js as sz_js' return sz_js = sz_js' -> (nat * nat) with
+             | [] => fun sz_js_nil => _
+             | a :: b =>
+               fun _ =>
+                 let slot' := check_slot (exist _ (a :: b) (cons_not_nil a b)) idx in
+                 let idx' := idx - (if eqb slot' 0
+                                    then 0
+                                    else strong_nth szs (slot' - 1) _)
+                 in (slot' , idx')
+             end) (eq_refl sz_js)).
+  (* sz_js <> [] *)
+  + assert(slot_lt : slot < length (combine szs (seq 0 (length szs)))).
+    { rewrite combine_length. rewrite seq_length. rewrite min_eq.
+      apply nooo with trs tr. apply tr_node. apply idx_lt_vec_len. }
+  (*   assert (length_sz_js_not_O : length sz_js_1 <> 0). *)
+  (*   { subst. unfold sz_js_1. rewrite combine_length. rewrite seq_length. *)
+  (*     rewrite min_eq. apply length_zero_iff_nil. apply szs_not_nil. } *)
+  (*   apply length_not_zero_inv in length_sz_js_not_O. *)
+  Admitted.
+
+Definition get {A : Set}
+   (tr : vector) (s : { idx : nat | (idx < @vec_length A tr) }) (default : A) : A.
+  refine ((match tr as tr' return tr = tr' -> A with
+           | Leaf szs ns => match s with
+                            | exist _ idx pf => fun tr => strong_nth ns idx _
+                            end
+           | Node ht szs trs => fun _ => default
+           end) (eq_refl tr)).
+  (* tr = Leaf .. *)
+  + rewrite vec_length_leaves_sizes with _ szs ns in pf.
+    - apply pf.
+    - apply tr.
+Defined.
+
+*)
+
+
+(*
+
+Lemma skipn_cons :
+  forall {A : Set} (m : nat) (xs : list A) (x : A),
+  length (skipn m (x :: xs)) = length (skipn m xs) + 1.
+Proof.
+  intros. induction m.
+  + simpl. omega.
+  + simpl. Admitted.
+(* Qed. *)
+
+Lemma length_not_empty_inv {A B : Set} :
+  forall (xs : list A) (ys : list B),
+  length xs = length ys -> xs <> [] -> ys <> [].
+Proof. Admitted.
+
+Lemma length_not_zero_inv {A : Set} :
+  forall (xs : list A),  length xs <> 0 -> xs <> [].
+Proof.
+  intros. induction xs.
+  + unfold length in H. congruence.
+  + apply (cons_not_empty a xs).
+Qed.
+
+Lemma length_zero_inv {A : Set} :
+  forall (xs : list A),  length xs = 0 -> xs = [].
+Proof.
+  intros. induction xs.
+  + reflexivity.
+  + apply length_zero_iff_nil. apply H.
+Qed.
+
+Lemma length_not_zero_inv_inv {A : Set} :
+  forall (xs : list A), xs <> [] -> length xs <> 0.
+Proof.
+  intros. induction xs.
+  + congruence.
+  + unfold length. apply Nat.neq_succ_0.
+Qed.
+
+Lemma skipn_length : forall {A : Set}
+  (ls : list A) (n : nat), length (skipn n ls) = length ls - n.
+Proof.
+  intros. induction ls.
+  + simpl. rewrite skipn_nil. reflexivity.
+  + rewrite skipn_cons.
+Admitted.
+
+Lemma skipn_not_nil : forall {A : Set}
+  (ls : list A) (n : nat), n < length ls -> ls <> [] -> skipn n ls <> [].
+Proof. Admitted.
+
+*)
